Syntax.v
@@ -7,11 +7,14 @@ Definition ident := string.
 Parameter atomic : Set.
 Parameter goal : Set.
 
+Inductive exception : Type :=
+| exn : string -> exception.
+
+Parameter unit : Set. 
+
 Inductive tactic : Type := 
 | single (a : atomic)
-(* | semicolon (t1 t2: tactic) *)
-(* | try (t1 : tactic) *)
-| zero (* todo: how to deal with thunking *)
-| plus (t1 t2 : tactic).
-(* | first (t1 : tactic) (t2 tactic_list). *)
-
+| zero (e : exception) (* Ltac2 Documentation: val zero : exn -> 'a*)
+| plus (t1 t2 : tactic) (*Ltac2 documentation: val plus
+ : (unit -> 'a) -> (exn -> 'a) -> 'a*)
+| throw (e : exception). (*ltac2 documentation: val throw : exn -> 'a*)
